version of the ideal CCA with sampling

theories/crypto/ICCA.ec
@@ -1,6 +1,8 @@
 require import AllCore List Distr DBool DInterval.
 require import Oracle_PKE.
 
+import Distr.MRat.
+
 (* Real/Ideal variant of IND-CCA2 *)
 
 theory ICCA.
@@ -19,7 +21,7 @@ op pkgen : keyseed -> pkey.
 op skgen : keyseed -> skey.
 op m0 : plaintext.
 
-axiom encK (k : keyseed) (m : plaintext) (e : encseed) : 
+axiom encK (k : keyseed) (m : plaintext) (e : encseed) :
   dec (enc(m, pkgen k, e), skgen k) = Some m.
 
 clone import CCA as C with
@@ -69,11 +71,11 @@ module Real : ICCA_Oracle = {
     var m;
 
     m <- dec(c, sk);
-    return m;    
+    return m;
   }
 }.
 
-module Ideal : ICCA_Oracle = { 
+module Ideal : ICCA_Oracle = {
   import var Real
   var cs : (ciphertext * plaintext) list
 
@@ -98,18 +100,62 @@ module Ideal : ICCA_Oracle = {
     cs <- (c, m) :: cs;
     return c;
   }
+
   proc dec (c : ciphertext) : plaintext option = {
     var m;
-    
+
     m <- assoc cs c;
-    if (m = None) { 
+    if (m = None) {
       m <- dec(c, sk);
     }
-    return m;    
+    return m;
   }
 }.
 
-module Real' : ICCA_Oracle = { 
+module Ideal' : ICCA_Oracle = {
+  import var Real
+  var n : int
+  var cs : (int * (ciphertext * plaintext)) list
+
+  proc init() : unit = {
+    var ks;
+
+    ks <$ dkeyseed;
+    pk <- pkgen ks;
+    sk <- skgen ks;
+    n <- 0;
+    cs <- [];
+  }
+
+  proc pk () = {
+    return pk;
+  }
+
+  proc enc (m : plaintext) : ciphertext = {
+    var e, c;
+
+    e <$ dencseed;
+    c <- enc(m0, pk, e);
+    n <- n + 1;
+    cs <- (n, (c, m)) :: cs;
+    return c;
+  }
+
+  proc dec (c : ciphertext) : plaintext option = {
+    var fcs, m, p;
+
+    fcs <- List.filter (fun p => fst (snd p) = c) cs;
+    if (fcs <> []) {
+      p <$ drat fcs;
+      m <- Some (snd (snd p));
+    } else {
+      m <- dec(c, sk);
+    }
+    return m;
+  }
+}.
+
+module Real' : ICCA_Oracle = {
   import var Real
   import var Ideal
 
@@ -134,14 +180,57 @@ module Real' : ICCA_Oracle = {
     cs <- (c, m) :: cs;
     return c;
   }
+
   proc dec (c : ciphertext) : plaintext option = {
     var m;
-    
+
     m <- assoc cs c;
-    if (m = None) { 
+    if (m = None) {
       m <- dec(c, sk);
     }
-    return m;    
+    return m;
+  }
+}.
+
+module Real'' : ICCA_Oracle = {
+  import var Real
+  import var Ideal'
+
+  proc init() : unit = {
+    var ks;
+
+    ks <$ dkeyseed;
+    pk <- pkgen ks;
+    sk <- skgen ks;
+    n <- 0;
+    cs <- [];
+  }
+
+  proc pk () = {
+    return pk;
+  }
+
+  proc enc (m : plaintext) : ciphertext = {
+    var e, c;
+
+    e <$ dencseed;
+    c <- enc(m, pk, e);
+    n <- n + 1;
+    cs <- (n, (c, m)) :: cs;
+    return c;
+  }
+
+  proc dec (c : ciphertext) : plaintext option = {
+    var fcs, m, p;
+
+    fcs <- List.filter (fun p => fst (snd p) = c) cs;
+    if (fcs <> []) {
+      p <$ drat fcs;
+      m <- Some (snd (snd p));
+    } else {
+      m <- dec(c, sk);
+    }
+    return m;
   }
 }.
 
@@ -150,10 +239,10 @@ module type Adversary (G : ICCA_Oracle) = {
 }.
 
 module Game (O : ICCA_i, A : Adversary) = {
-  
+
   proc main() = {
     var r;
-    
+
     O.init();
     r <@ A(O).main();
     return r;
@@ -173,7 +262,7 @@ module CountICCA (O : ICCA_Oracle) = {
   proc pk = O.pk
 
   proc enc (m : plaintext) : ciphertext = {
-    var c; 
+    var c;
 
     c <@ O.enc(m);
     nenc <- nenc + 1;
@@ -181,7 +270,7 @@ module CountICCA (O : ICCA_Oracle) = {
   }
 
   proc dec (c : ciphertext) : plaintext option = {
-    var m; 
+    var m;
 
     m <@ O.dec(c);
     ndec <- ndec + 1;
@@ -238,9 +327,54 @@ module B (A : Adversary) (O : CCA_Oracle) = {
   }
 }.
 
+module B' (A : Adversary) (O : CCA_Oracle) = {
+  var n : int
+  var cs : (int * (ciphertext * plaintext)) list
+  var pk : pkey
+
+  module O' : ICCA_Oracle = {
+
+    proc init (p : pkey) = { pk <- p; }
+
+    proc pk () = { return pk; }
+
+    proc enc (m : plaintext) = {
+      var c;
+
+      c <- O.l_or_r(m, m0);
+      n <- n + 1;
+      cs <- (n, (c, m)) :: cs;
+      return c;
+    }
+
+    proc dec (c : ciphertext) : plaintext option = {
+      var fcs, m, p;
+
+      fcs <- List.filter (fun p => fst (snd p) = c) cs;
+      if (fcs <> []) {
+        p <$ drat fcs;
+        m <- Some (snd (snd p));
+      } else {
+        m <- O.dec(c);
+      }
+      return m;
+    }
+  }
+
+  proc main (pk : pkey) : bool = {
+    var r;
+
+    n <- 0;
+    cs <- [];
+    O'.init(pk);
+    r <@ A(O').main();
+    return r;
+  }
+}.
+
 section.
 
-declare module A : Adversary {Real, Real', Ideal, C.Wrap, B, CountCCA, CountICCA}.
+declare module A : Adversary {Real, Real', Ideal, Ideal', C.Wrap, B, B', CountCCA, CountICCA}.
 
 axiom A_bound (O <: ICCA_Oracle {A, CountICCA}) : hoare [CountAdv(A, O).main :
                true ==> CountICCA.ndec <= Ndec /\ CountICCA.nenc <= Nenc].
@@ -254,10 +388,10 @@ proc. inline*; sp; auto.
 call (: ={glob O, glob B} /\ CountCCA.ndec{1} <= CountICCA.ndec{2} /\
         CountCCA.nenc{1} = CountICCA.nenc{2}) => //.
 - by proc; auto.
-- proc; inline *; sp; auto; call (: true); auto => /> /#.
+- by proc; inline *; sp; auto; call (: true); auto => /> /#.
 - proc; inline *; sp; auto.
   if; auto => />; 2: by smt().
-  sp; call (: true); auto => /> /#.
+  by sp; call (: true); auto => /> /#.
 qed.
 
 lemma B_bound (O <: CCA_Oracle{CountCCA, CountICCA, A, B}) :
@@ -270,15 +404,34 @@ qed.
 equiv Real_Real' :
   Game(Real, A).main ~ Game(Real', A).main : ={glob A} ==> ={res}.
 proof.
-proc; inline *. 
+proc; inline *.
 call (: ={glob Real} /\ (exists ks, (Real.pk, Real.sk){2} = (pkgen ks, skgen ks)) /\
-  (forall c m, assoc Ideal.cs c = Some m => dec(c, Real.sk) = Some m){2}).
-- proc; auto.
-- proc. wp; rnd; auto=> /> &m2 ks Hcs e _ c m'.
+        (forall c m, assoc Ideal.cs c = Some m => dec(c, Real.sk) = Some m){2}).
+- by proc; auto.
+- proc; wp; rnd; auto=> /> &m2 ks Hcs e _ c m'.
   rewrite assoc_cons. case: (c = enc (m{m2}, pkgen ks, e)) => />; 1: by rewrite encK.
-  move => _; apply: Hcs.
-- proc. wp. skip => /> &m2 ks Hcs /#.
-- wp; rnd; skip => /> /#.
+  by move => _; apply: Hcs.
+- by proc; wp; skip => /> &m2 ks Hcs /#.
+- by wp; rnd; skip => /> /#.
+qed.
+
+equiv Real_Real'' :
+  Game(Real, A).main ~ Game(Real'', A).main : ={glob A} ==> ={res}.
+proof.
+proc; inline *.
+call (: ={glob Real} /\ (exists ks, (Real.pk, Real.sk){2} = (pkgen ks, skgen ks)) /\
+        (forall c p, p \in drat (List.filter (fun p => fst (snd p) = c) Ideal'.cs) =>
+                     dec(c, Real.sk) = Some (snd (snd p))){2}).
+- by proc; auto.
+- proc; wp; rnd; auto => /> &m2 ks csP e ? c ?.
+  case: (enc (m{m2}, pkgen ks, e) = c); 2: by move => _; apply csP.
+  rewrite supp_drat in_cons.
+  move => ? [|]; 1: smt(encK).
+  by rewrite -supp_drat; apply csP.
+- proc; sp; if{2}; 2: by auto => />.
+  auto => /> &m2 ks Hcs fP; split; 1: smt(drat_ll).
+  by move => _; apply Hcs.
+- by wp; rnd; skip => />; smt(supp_drat).
 qed.
 
 module S : Scheme = {
@@ -312,15 +465,38 @@ equiv Real'_CCA_L :
 proof.
 proc; inline *; wp.
 call (: ={pk, sk}(Real, Wrap) /\ unzip1 Ideal.cs{1} = Wrap.cs{2} /\
-      (forall c m, assoc Ideal.cs c = Some m => dec(c, Real.sk) = Some m){1} /\ 
-      (exists ks, (Wrap.pk, Wrap.sk){2} = (pkgen ks, skgen ks)) /\ 
-      Ideal.cs{1} = B.cs{2} /\ B.pk{2} = Wrap.pk{2}).
+        (forall c m, assoc Ideal.cs c = Some m => dec(c, Real.sk) = Some m){1} /\
+        (exists ks, (Wrap.pk, Wrap.sk){2} = (pkgen ks, skgen ks)) /\
+        Ideal.cs{1} = B.cs{2} /\ B.pk{2} = Wrap.pk{2}).
 - by proc; inline *; auto => />.
-- proc; inline *; auto => /> &m1 &m2 Hcs ks ? ? e _ c m'. 
-  rewrite assoc_cons; case : (c = enc (m{m2}, pkgen ks, e)) => />; smt(encK).
-- proc; inline *; auto => /> &m1 &m2 Hcs ks ? ?. 
+- proc; inline *; auto => /> &m1 &m2 Hcs ks ? ? e _ c m'.
+  by rewrite assoc_cons; case : (c = enc (m{m2}, pkgen ks, e)) => />; smt(encK).
+- proc; inline *; auto => /> &m1 &m2 Hcs ks ? ?.
   by rewrite -assocTP.
-- wp; rnd; skip => /> /#.
+- by wp; rnd; skip => /> /#.
+qed.
+
+equiv Real''_CCA_L :
+  Game(Real'', A).main ~ CCA_L(S, B'(A)).main : ={glob A} ==> ={res}.
+proof.
+proc; inline *; wp.
+call (: ={pk, sk}(Real,Wrap) /\ unzip1 (unzip2 Ideal'.cs{1}) = Wrap.cs{2} /\
+        (forall c i m, (i, (c, m)) \in List.filter (fun p => fst (snd p) = c)
+                                                   Ideal'.cs =>
+                       dec(c, Real.sk) = Some m){1} /\
+        (exists ks, (Wrap.pk, Wrap.sk){2} = (pkgen ks, skgen ks)) /\
+        Ideal'.cs{1} = B'.cs{2} /\ B'.pk{2} = Wrap.pk{2} /\
+        Ideal'.n{1} = B'.n{2}).
+- by proc; inline *; auto => />.
+- proc; inline *; auto => /> &m1 &m2 Hcs ks skP ? e _ c i ?.
+  case: (enc (m{m2}, pkgen ks, e) = c).
+  + move => ? [|?]; 1: smt(encK).
+    by rewrite -skP; apply (Hcs c i); smt().
+  + by move => _ ?; rewrite -skP; apply (Hcs c i); smt().
+- proc; inline *; sp; auto; if; auto => /> &m1 &m2 Hcs ks ? ? csP.
+  rewrite mem_map_fst; move => [?].
+  rewrite mem_map_snd; smt(mem_filter).
+- by wp; rnd; skip => /> /#.
 qed.
 
 equiv Ideal_CCA_R :
@@ -328,15 +504,36 @@ equiv Ideal_CCA_R :
 proof.
 proc; inline *; wp.
 call (: ={pk, sk}(Real,Wrap) /\ unzip1 Ideal.cs{1} = Wrap.cs{2} /\
-      (forall c m, assoc Ideal.cs c = Some m => dec(c, Real.sk) = Some m0){1} /\ 
-      (exists ks, (Wrap.pk, Wrap.sk){2} = (pkgen ks, skgen ks)) /\ 
-      Ideal.cs{1} = B.cs{2} /\ B.pk{2} = Wrap.pk{2}).
+        (forall c m, assoc Ideal.cs c = Some m => dec(c, Real.sk) = Some m0){1} /\
+        (exists ks, (Wrap.pk, Wrap.sk){2} = (pkgen ks, skgen ks)) /\
+        Ideal.cs{1} = B.cs{2} /\ B.pk{2} = Wrap.pk{2}).
 - by proc; inline *; auto => />.
 - proc; inline *; auto => /> &m1 &m2 Hcs ks ? ? e _ c m'.
-  rewrite assoc_cons; case : (c = enc (m0, pkgen ks, e)) => />; smt(encK).
-- proc; inline *; auto => /> &m1 &m2 Hcs ks ? ?. 
+  by rewrite assoc_cons; case : (c = enc (m0, pkgen ks, e)) => />; smt(encK).
+- proc; inline *; auto => /> &m1 &m2 Hcs ks ? ?.
   by rewrite -assocTP.
-- wp; rnd; skip => /> /#.
+- by wp; rnd; skip => /> /#.
+qed.
+
+equiv Ideal'_CCA_R :
+  Game(Ideal', A).main ~ CCA_R(S, B'(A)).main : ={glob A} ==> ={res}.
+proof.
+proc; inline *; wp.
+call (: ={pk, sk}(Real,Wrap) /\ unzip1 (unzip2 Ideal'.cs{1}) = Wrap.cs{2} /\
+        (forall c i m, (i, (c, m)) \in List.filter (fun p => fst (snd p) = c)
+                                                   Ideal'.cs =>
+                       dec(c, Real.sk) = Some m0){1} /\
+        (exists ks, (Wrap.pk, Wrap.sk){2} = (pkgen ks, skgen ks)) /\
+        Ideal'.cs{1} = B'.cs{2} /\ B'.pk{2} = Wrap.pk{2} /\
+        Ideal'.n{1} = B'.n{2}).
+- by proc; inline *; auto => />.
+- proc; inline *; auto => /> &m1 &m2 Hcs ks skP ? e _ c i m'.
+  case: (enc (m0, pkgen ks, e) = c); 1: smt(encK).
+  by move => _ ?; rewrite -skP; apply (Hcs c i m'); smt().
+- proc; inline *; sp; auto; if; auto => /> &m1 &m2 Hcs ks ? ? csP.
+  rewrite mem_map_fst; move => [?].
+  rewrite mem_map_snd; smt(mem_filter).
+- by wp; rnd; skip => /> /#.
 qed.
 
 lemma ICCA_CCALR &m :
@@ -349,6 +546,18 @@ have -> : Pr[Game(Real', A).main() @ &m : res] = Pr[CCA_L(S, B(A)).main() @ &m :
 - byequiv => //; conseq (: ={glob A} ==> ={res}) => //; exact Real'_CCA_L.
 have -> : Pr[Game(Ideal, A).main() @ &m : res] = Pr[CCA_R(S, B(A)).main() @ &m : res]; 2: by smt().
 byequiv => //; conseq (: ={glob A} ==> ={res}) => //; exact Ideal_CCA_R.
+qed.
+
+lemma ICCA_CCALR' &m :
+  Pr[Game(Real, A).main() @ &m : res] - Pr[Game(Ideal', A).main() @ &m : res] =
+  Pr[CCA_L(S, B'(A)).main() @ &m : res] - Pr[CCA_R(S, B'(A)).main() @ &m : res].
+proof.
+have -> : Pr[Game(Real, A).main() @ &m : res] = Pr[Game(Real'', A).main() @ &m : res].
+- byequiv => //; conseq (: ={glob A} ==> ={res}) => //; exact Real_Real''.
+have -> : Pr[Game(Real'', A).main() @ &m : res] = Pr[CCA_L(S, B'(A)).main() @ &m : res].
+- byequiv => //; conseq (: ={glob A} ==> ={res}) => //; exact Real''_CCA_L.
+have -> : Pr[Game(Ideal', A).main() @ &m : res] = Pr[CCA_R(S, B'(A)).main() @ &m : res]; 2: by smt().
+byequiv => //; conseq (: ={glob A} ==> ={res}) => //; exact Ideal'_CCA_R.
 qed.
 
 end section.
