theories/crypto/Oracle_PKE.ec
@@ -11,15 +11,15 @@ require (*--*) LorR Hybrid.
 
 type ('a, 'b) sum = [Left of 'a | Right of 'b].
 
-op is_left ['a 'b] (s : ('a,'b) sum) = 
+op is_left ['a 'b] (s : ('a,'b) sum) =
   with s = Left _ => true
   with s = Right _ => false.
 
-op left ['a 'b] (s : ('a,'b) sum) = 
+op left ['a 'b] (s : ('a,'b) sum) =
   with s = Left x => x
   with s = Right _ => witness.
 
-op right ['a 'b] (s : ('a,'b) sum) = 
+op right ['a 'b] (s : ('a,'b) sum) =
   with s = Right x => x
   with s = Left _ => witness.
 
@@ -61,7 +61,7 @@ module type Adversary (O : CCA_Oracle) = {
   proc main (pk : pkey) : bool
 }.
 
-module type LR = { 
+module type LR = {
   proc init () : unit
   proc l_or_r (m0 m1 : plaintext) : plaintext
 }.
@@ -69,29 +69,29 @@ module type LR = {
 module LorR : LR = {
   var b : bool
 
-  proc init () = { 
+  proc init () = {
     b <$ {0,1};
   }
 
   proc l_or_r (m0 m1 : plaintext) = {
     return b?m0:m1;
-  } 
+  }
 }.
 
 module L : LR = {
-  proc init () = { } 
+  proc init () = { }
 
   proc l_or_r (m0 m1 : plaintext) = {
     return m0;
-  } 
+  }
 }.
 
 module R : LR = {
-  proc init () = { } 
+  proc init () = { }
 
   proc l_or_r (m0 m1 : plaintext) = {
     return m1;
-  } 
+  }
 }.
 
 (* Oracles for CCA games *)
@@ -106,7 +106,7 @@ module Wrap (S : Scheme, LR : LR) : CCA_Oracle_i = {
     (pk, sk) <@ S.kg();
     cs <- [];
   }
-  
+
   proc l_or_r (m0 m1 : plaintext) : ciphertext = {
     var c, m;
 
@@ -115,10 +115,10 @@ module Wrap (S : Scheme, LR : LR) : CCA_Oracle_i = {
     cs <- c :: cs;
     return c;
   }
-  
+
   proc dec (c : ciphertext) : plaintext option = {
     var m;
-    
+
     m <- witness;
     if (! c \in cs) {
       m <- S.dec(sk, c);
@@ -133,10 +133,10 @@ module CountCCA (O : CCA_Oracle) = {
   proc init () : unit = {
     ndec <- 0;
     nenc <- 0;
-  } 
+  }
 
   proc l_or_r (m0 m1 : plaintext) : ciphertext = {
-    var c; 
+    var c;
 
     c <@ O.l_or_r(m0, m1);
     nenc <- nenc + 1;
@@ -144,7 +144,7 @@ module CountCCA (O : CCA_Oracle) = {
   }
 
   proc dec (c : ciphertext) : plaintext option = {
-    var m; 
+    var m;
 
     m <@ O.dec(c);
     ndec <- ndec + 1;
@@ -162,10 +162,10 @@ module CountAdv (A : Adversary) (O : CCA_Oracle) = {
   }
 }.
 
-(** Plan: 
+(** Plan:
     1. Create Wraper for Adversaries that does (only) the counting
-    2. Remove counting from Wrap 
-    3. CCA games call wrapped/restricted adversaries 
+    2. Remove counting from Wrap
+    3. CCA games call wrapped/restricted adversaries
     4. express A_bound using counting wrapper
     5. A' used restricted adversary (and so satisfies call restrictions) *)
 
@@ -197,13 +197,13 @@ module B (S : Scheme, A : Adversary, O : CCA_Oracle) = {
   var i, iS : int
   var pk : pkey
   var cs : ciphertext list
-  
+
   module O' : CCA_Oracle = {
     proc l_or_r (m0 m1 : plaintext) = {
       var c;
 
       if (iS < i) c <- S.enc(pk, m0);
-      else { 
+      else {
         if (i = iS) c <- O.l_or_r(m0, m1);
         else c <- S.enc(pk, m1);
       }
@@ -238,7 +238,7 @@ section.
 declare module S : Scheme {Wrap, LorR, B, CountCCA, CountAdv}.
 declare module A : Adversary {Wrap, S, LorR, B, CountCCA, CountAdv}.
 
-axiom A_ll (O <: CCA_Oracle {A}) : 
+axiom A_ll (O <: CCA_Oracle {A}) :
   islossless O.l_or_r => islossless O.dec => islossless A(O).main.
 
 axiom kg_ll : islossless S.kg.
@@ -253,11 +253,11 @@ local clone Hybrid as Hyb with
   type outputA <- bool,
   op q <- Nenc.
 
-axiom A_bound (O <: CCA_Oracle {A, CountCCA}): 
+axiom A_bound (O <: CCA_Oracle {A, CountCCA}) :
   hoare[ CountAdv(A, O).main : true ==> CountCCA.ndec <= Ndec /\ CountCCA.nenc <= Nenc].
 
-lemma A_bound' (O <: CCA_Oracle {A, CountCCA}): 
-  hoare[ A(CountCCA(O)).main : 
+lemma A_bound' (O <: CCA_Oracle {A, CountCCA}) :
+  hoare[ A(CountCCA(O)).main :
     CountCCA.ndec = 0 /\ CountCCA.nenc = 0 ==> CountCCA.ndec <= Ndec /\ CountCCA.nenc <= Nenc].
 proof.
 suff E : equiv [A(CountCCA(O)).main ~ CountAdv(A, O).main :
@@ -268,20 +268,20 @@ suff E : equiv [A(CountCCA(O)).main ~ CountAdv(A, O).main :
   by skip => />.
 qed.
 
-lemma CCA_LR &m : 
-  `| Pr[ CCA(S, A).main() @ &m : res] - 1.0/2.0 | = 
+lemma CCA_LR &m :
+  `| Pr[ CCA(S, A).main() @ &m : res] - 1.0/2.0 | =
   1%r / 2%r * `| Pr[ CCA_L(S, A).main() @ &m : res ] - Pr[ CCA_R(S, A).main() @ &m : res ] |.
 proof.
   rewrite (Top.LorR.pr_AdvLR_AdvRndLR (CCA_L(S, A)) (CCA_R(S, A)) &m).
-    byphoare => //. 
+    byphoare => //.
     islossless; last by apply: kg_ll.
-    apply: (A_ll(CountCCA(Wrap(S, R)))); first by islossless; apply: enc_ll. 
+    apply: (A_ll(CountCCA(Wrap(S, R)))); first by islossless; apply: enc_ll.
     islossless; apply: dec_ll.
-  suff <- : Pr[CCA(S, A).main() @ &m : res] = 
+  suff <- : Pr[CCA(S, A).main() @ &m : res] =
             Pr[Top.LorR.RandomLR(CCA_L(S, A),CCA_R(S, A)).main() @ &m : res] by smt().
   byequiv=> //. proc; inline *.
   seq 1 1 : (={glob A,glob S} /\ LorR.b{1} = b{2}); first by rnd.
-  if{2}; wp. 
+  if{2}; wp.
   - call (: ={glob S, glob Wrap} /\ LorR.b{1}).
     + by proc; inline *; sp; auto; call (: true); auto => />.
     + by sim / (LorR.b{1}) : (={res,glob S, glob Wrap}).
@@ -299,7 +299,7 @@ local module LRB (O : CCA_Oracle) : CCA_Oracle = {
     var c;
 
     if (iS < i) c <- S.enc(pk, m0);
-    else { 
+    else {
       if (i = iS) c <- O.l_or_r(m0, m1);
       else c <- S.enc(pk, m1);
     }
@@ -317,7 +317,7 @@ local module LRB (O : CCA_Oracle) : CCA_Oracle = {
   }
 }.
 
-lemma B_bound (O <: CCA_Oracle {S, CountCCA, A, B}): 
+lemma B_bound (O <: CCA_Oracle {S, CountCCA, A, B}) :
   hoare[ CountAdv(B(S, A), O).main : true ==> CountCCA.ndec <= Ndec /\ CountCCA.nenc <= 1].
 proof.
 proc; inline *; swap 5 -2; sp; auto.
@@ -330,7 +330,7 @@ proc; inline *; swap 5 -2; sp; auto.
     wp; sp; call (: true); skip; smt().
   + by conseq />.
   + auto => />; smt(supp_dinter).
-- call (: CountCCA.ndec = 0 ==> CountCCA.ndec <= Ndec); 2: auto. 
+- call (: CountCCA.ndec = 0 ==> CountCCA.ndec <= Ndec); 2: auto.
   suff E : equiv[ A(B(S, A, CountCCA(O)).O').main ~ A(CountCCA(LRB(O))).main :
            ={glob O, glob S, glob A, B.iS, B.i, B.pk, CountCCA.ndec, pk} /\
            CountCCA.ndec{1} = 0 /\
@@ -375,15 +375,15 @@ local module Ob : Hyb.Orclb = {
     }
     return ol;
   }
-  
-  proc orclL (m0 m1 : plaintext) : ciphertext = { 
+
+  proc orclL (m0 m1 : plaintext) : ciphertext = {
     var c;
 
     c <@ S.enc(pk, m0);
     cs <- c :: cs;
     return c;
   }
-  
+
   proc orclR (m0 m1 : plaintext) : ciphertext = {
     var c;
 
@@ -414,11 +414,11 @@ local module A' (Ob : Hyb.Orclb) (O : Hyb.Orcl) = {
     proc l_or_r = O.orcl
 
     proc dec (c : ciphertext) : plaintext option = {
-      var m; 
+      var m;
 
       m <@ Ob.leaks(Right c);
       return right m;
-    } 
+    }
   }
 
   proc main() : bool = {
@@ -431,7 +431,7 @@ local module A' (Ob : Hyb.Orclb) (O : Hyb.Orcl) = {
   }
 }.
 
-local lemma A'_ll (Ob <: Hyb.Orclb{A'}) (LR <: Hyb.Orcl{A'}) : 
+local lemma A'_ll (Ob <: Hyb.Orclb{A'}) (LR <: Hyb.Orcl{A'}) :
   islossless LR.orcl => islossless Ob.leaks =>
   islossless Ob.orclL => islossless Ob.orclR =>
   islossless A'(Ob, LR).main.
@@ -440,24 +440,24 @@ proof.
   apply (A_ll (<: CountCCA(A'(Ob, LR).O'))); islossless.
 qed.
 
-local lemma CCA_Ln &m : 
+local lemma CCA_Ln &m :
    Pr[ CCA_L(S, A).main() @ &m : res ] = Pr[ Hyb.Ln(Ob, A').main() @ &m : res ].
 proof.
   byequiv => //; proc. inline *; sp; wp; rcondt{2} 1 => //.
   call (: ={glob S} /\ ={sk, pk, cs}(Wrap,Ob)).
-  + proc; auto; inline *; auto. 
+  + proc; auto; inline *; auto.
     by call (: true); auto => />.
   + proc; auto; inline *. sp; rcondf{2} 1 => //; sp.
     by if; 1: smt(); auto; call (: true).
   + by auto; call(: true).
 qed.
 
-local lemma CCA_Rn &m : 
+local lemma CCA_Rn &m :
    Pr[ CCA_R(S, A).main() @ &m : res ] = Pr[ Hyb.Rn(Ob, A').main() @ &m : res].
 proof.
   byequiv => //; proc. inline *; sp; wp; rcondt{2} 1 => //.
   call (: ={glob S} /\ ={sk,pk,cs}(Wrap,Ob)).
-  + proc; auto; inline *; auto. 
+  + proc; auto; inline *; auto.
     by call (: true); auto => />.
   + proc; auto; inline *. sp; rcondf{2} 1 => //; sp.
     by if; 1: smt(); auto; call (: true).
@@ -484,21 +484,21 @@ import StdOrder.RealOrder.
 
 lemma CCA_1n &m :
     `| Pr[ CCA_L(S, A).main() @ &m : res ] - Pr[ CCA_R(S, A).main() @ &m : res ] |
-    <= 
+    <=
     Nenc%r * `| Pr[ CCA_L(S,B(S, A)).main() @ &m : res ] - Pr[ CCA_R(S,B(S, A)).main() @ &m : res ] |.
 proof.
 rewrite -ler_pdivr_mull; 1: smt(Nenc_gt0).
-have -> : inv Nenc%r * `|Pr[CCA_L(S, A).main() @ &m : res] - Pr[CCA_R(S, A).main() @ &m : res]| = 
+have -> : inv Nenc%r * `|Pr[CCA_L(S, A).main() @ &m : res] - Pr[CCA_R(S, A).main() @ &m : res]| =
           `| (Pr[ CCA_L(S, A).main() @ &m : res ] - Pr[ CCA_R(S, A).main() @ &m : res]) / Nenc%r |.
 smt(Nenc_gt0).
-rewrite CCA_Ln CCA_Rn. 
+rewrite CCA_Ln CCA_Rn.
 have /= H := Hyb.Hybrid_restr Ob A' A'_call Obl_ll orclL_ll orclR_ll A'_ll &m (fun _ _ _ r => r).
 rewrite -H; clear H.
 have <- : Pr[CCA_(S, B(S, A), L).main() @ &m : res] = Pr[Hyb.HybGame(A', Ob, Hyb.L(Ob)).main() @ &m : res].
-  byequiv => //; proc; inline *; auto. 
-  swap{2} 1 5; swap{1} 6 2; sp. 
+  byequiv => //; proc; inline *; auto.
+  swap{2} 1 5; swap{1} 6 2; sp.
   rcondt{2} 1; 1: by move => &m'; skip => />.
-  call (: ={glob S} /\ ={pk, sk}(Wrap, Ob) /\ 
+  call (: ={glob S} /\ ={pk, sk}(Wrap, Ob) /\
             B.i{1} = Hyb.HybOrcl.l{2} /\ B.iS{1} = Hyb.HybOrcl.l0{2} /\ ={cs, pk}(B, Ob) /\
             (forall c, c \in Wrap.cs{1} => c \in B.cs{1})).
   - proc; auto; inline *; sp; if; 1: by move => />.
@@ -507,16 +507,16 @@ have <- : Pr[CCA_(S, B(S, A), L).main() @ &m : res] = Pr[Hyb.HybGame(A', Ob, Hyb
       * by auto; call(: true); auto => /> /#.
       * by auto; call(: true); auto => /> /#.
   - proc; inline *; sp. rcondf{2} 1; 1: by move => &m'; skip => />.
-    sp. if; 1: by move => &m1 &m2 />. 
-    + sp. rcondt{1} 1. move => &m1; skip => /> /#. 
+    sp. if; 1: by move => &m1 &m2 />.
+    + sp. rcondt{1} 1. move => &m1; skip => /> /#.
       by auto; call(: true); skip => />.
     + by auto; skip => />.
   by wp; rnd; auto; call(: true); skip => &m1 &m2 />.
 have <- : Pr[CCA_(S, B(S, A), R).main() @ &m : res] = Pr[Hyb.HybGame(A', Ob, Hyb.R(Ob)).main() @ &m : res].
-  byequiv => //; proc; inline *; auto. 
-  swap{2} 1 5; swap{1} 6 2; sp. 
+  byequiv => //; proc; inline *; auto.
+  swap{2} 1 5; swap{1} 6 2; sp.
   rcondt{2} 1; 1: by move => &m'; skip => />.
-  call (: ={glob S} /\ ={pk,sk}(Wrap,Ob) /\ 
+  call (: ={glob S} /\ ={pk,sk}(Wrap,Ob) /\
             B.i{1} = Hyb.HybOrcl.l{2} /\ B.iS{1} = Hyb.HybOrcl.l0{2} /\ ={cs,pk}(B,Ob) /\
             (forall c, c \in Wrap.cs{1} => c \in B.cs{1})).
   - proc; auto; inline *; sp; if; 1: by move => />.
@@ -525,8 +525,8 @@ have <- : Pr[CCA_(S, B(S, A), R).main() @ &m : res] = Pr[Hyb.HybGame(A', Ob, Hyb
       * by auto; call(: true); auto => /> /#.
       * by auto; call(: true); auto => /> /#.
   - proc; inline *; sp. rcondf{2} 1; 1: by move => &m'; skip => />.
-    sp. if; 1: by move => &m1 &m2 />. 
-    + sp. rcondt{1} 1. move => &m1; skip => /> /#. 
+    sp. if; 1: by move => &m1 &m2 />.
+    + sp. rcondt{1} 1. move => &m1; skip => /> /#.
       by auto; call(: true); skip => />.
     + by auto; skip => />.
   by wp; rnd; auto; call(: true); skip => &m1 &m2 />.
@@ -536,4 +536,3 @@ qed.
 end section.
 
 end CCA.
-
